\documentclass{article}
\usepackage{amsmath}

\begin{document}

\begin{align*} 
    A) \ \ & \Sigma = \{a, 0, 1\} \text{ and } L = \{ \text{ if } n \text{ even: } x = 0 \text{ else: } x = 1\}.\\
    B) \ \ & \{w \in \{a, b\}^* \mid w \text{ not contains the subword } abba\}.\\
    C) \ \ & L = \{w \in \{a, b, c, d\}^* \mid |w|_a \geq 1 \text{ and } |w|_b \geq 1 \text{ and } |w|_c \geq 1\}.\\
    D) \ \ & \text{regular grammar} \ \  G= (\{S,\,A,\,B,\,C\}, \{a,\,b\},\, P,\, S) \text{ with }\\
    & \hspace*{30mm} \mathcla{
        \begin{align*}
            P = \{ S & \rightarrow \epsilon \mid aS \mid bB \mid B\\
            B & \rightarrow bB \mid aA \mid A \\
            A & \rightarrow bS \mid aC \\
            C & \rightarrow aC \mid bC \mid a \mid b\}.\\
        \end{align*}}\\
    E) \ \ & \text{regular grammar} \ \  G= (\{S,\,A,\,B,\,C\}, \{a,\,b\},\, P,\, S) \text{ with }\\
    & \hspace*{30mm} \mathcla{
        \begin{align*}
           P = \{  S & \rightarrow \epsilon \mid aA\\
           A & \rightarrow aA \mid bB\\
           B & \rightarrow bB \mid aC\\
           C & \rightarrow bA \mid aB \mid b\}.
        \end{align*}}\\
    F) \ \  & \Sigma = \{a, 0, 1\} \text{ and } L = \{ w \in \Sigma^* \mid \text{ there are } u_1, u_2, u_3 \in \Gamma^* \text{ with } \vert u_2 \vert = 3, \text{ so that } w= u_1 a u_2 b u_3  \}
\end{align*}

\end{document}